progs/verif_message.v
@@ -14,39 +14,71 @@ Require Import progs.message.
 
 Local Open Scope logic.
 
+
+Lemma typed_mapsto_typed_mapsto_ :
+  forall sh t v v', typed_mapsto sh t v v' |-- typed_mapsto_ sh t v.
+Admitted.
+Hint Resolve typed_mapsto_typed_mapsto_.
+Hint Resolve field_mapsto_field_mapsto_.
+
+
 (* message_format t = (length, f)
    where 
     f sh buf data  := the [data] is formatted into a message 
          at most [length] bytes, 
           stored starting at address [buf] with share [sh] *)
-Definition message_format (t: type) : Type :=
-   (Z * (forall (sh: share) (buf: val) (data: reptype t), mpred))%type.
 
-Definition intpair_message: message_format t_struct_intpair :=
-  (8, typed_mapsto t_struct_intpair).
+Record message_format (t: type) : Type :=
+mf_build {
+   mf_size: Z;
+   mf_assert: forall (sh: share) (buf: val) (len: Z) (data: reptype t), mpred;
+   mf_bufprop: forall sh buf len data, 
+           mf_assert sh buf len data |-- 
+                 !!(0 <= len <= mf_size) && memory_block sh (Int.repr len) buf;
+   mf_restbuf := fun (sh: share) (buf: val) (len: Z) => 
+                              memory_block sh (Int.repr (mf_size-len)) (offset_val buf (Int.repr len))
+}.
+
+Implicit Arguments mf_build [[t]].
+Implicit Arguments mf_size [[t]].
+Implicit Arguments mf_assert [[t]].
+Implicit Arguments mf_bufprop [[t]].
+Implicit Arguments mf_restbuf [[t]].
+(* need to add a proof to message_format, that the
+     representation of a  buf implies the typed_mapsto_ of the bufsize array *)
+
+ 
+Program Definition intpair_message: message_format t_struct_intpair :=
+  mf_build 8 (fun sh buf len data => !!(len=8) && typed_mapsto sh t_struct_intpair buf data) _.
+Next Obligation.
+ normalize. repeat apply andp_right; try (apply prop_right; compute; congruence).
+ change 8 with (sizeof t_struct_intpair). rewrite memory_block_typed. auto.
+Qed.
 
 Definition serialize_spec {t: type} (format: message_format t) :=
   WITH data: reptype t, p: val, buf: val, sh: share, sh': share
   PRE [ _p OF (tptr t), _buf OF (tptr tuchar) ] 
           PROP (writable_share sh')
           LOCAL (`(eq p) (eval_id _p); `(eq buf) (eval_id _buf))
-          SEP (`(typed_mapsto t sh p data); 
-                 `(memory_block sh' (Int.repr (fst format)) buf))
+          SEP (`(typed_mapsto sh t p data); 
+                 `(memory_block sh' (Int.repr (mf_size format)) buf))
   POST [ tint ]  
-          local (`(fun len => 0 <= Int.signed (force_int len) <= fst format) retval) &&
-         `(typed_mapsto t sh p data)  * `(snd format sh' buf) `data.
+         EX len: Z, 
+          local (`(eq (Vint (Int.repr len))) retval) &&
+         `(typed_mapsto sh t p data)  
+            * `(mf_assert format sh' buf len data) * `(mf_restbuf format sh' buf len).
 
 Definition deserialize_spec {t: type} (format: message_format t) :=
   WITH data: reptype t, p: val, buf: val, shs: share*share, len: Z
   PRE [ _p OF (tptr t), _buf OF (tptr tuchar), _length OF tint ] 
-          PROP (writable_share (fst shs); 0 <= len <= fst format)
+          PROP (writable_share (fst shs); 0 <= len <= mf_size format)
           LOCAL (`(eq p) (eval_id _p); `(eq buf) (eval_id _buf);
                         `(eq (Vint (Int.repr len))) (eval_id _length))
-          SEP (`(snd format (snd shs) buf) `data;
-                 `(memory_block (fst shs) (Int.repr (fst format)) p))
+          SEP (`(mf_assert format (snd shs) buf len data);
+                 `(memory_block (fst shs) (Int.repr (mf_size format)) p))
   POST [ tint ]
-            `(snd format (snd shs) buf data) *
-            `(typed_mapsto t (fst shs) p data).
+            `(mf_assert format (snd shs) buf len data) *
+            `(typed_mapsto (fst shs) t p data).
 
 Definition intpair_serialize_spec :=
  DECLARE _intpair_serialize (serialize_spec intpair_message).
@@ -62,11 +94,11 @@ Definition main_spec :=
 
 Definition Vprog : varspecs := (_intpair_message, t_struct_message)::nil.
 
-Definition message {t: type} (format: message_format t) (sh: share) (m: val) : mpred :=
+Definition message (sh: share) {t: type} (format: message_format t) (m: val) : mpred :=
   EX fg: val*val,
           func_ptr (serialize_spec format) (fst fg) &&
           func_ptr (deserialize_spec format) (snd fg) &&
-       typed_mapsto t_struct_message sh m (Int.repr (fst format), (fst fg, snd fg)).
+       typed_mapsto sh t_struct_message m (Int.repr (mf_size format), (fst fg, snd fg)).
 
 Definition Gprog : funspecs := 
     intpair_serialize_spec :: intpair_deserialize_spec :: main_spec::nil.
@@ -82,7 +114,7 @@ name p0 _p.
 name buf0 _buf.
 name x _x.
 name y _y.
-change (fst intpair_message) with (sizeof t_struct_intpair).
+change (mf_size intpair_message) with (sizeof t_struct_intpair).
 rewrite memory_block_typed.
 do 2 simpl_typed_mapsto.
 destruct data as (x1,y1); simpl in *.
@@ -108,10 +140,8 @@ forward. (*  ((int * )buf)[1]=y; *)
 go_lower. subst. apply andp_right; auto. apply prop_right; intuition.
 forward. (* return 8; *)
 go_lower. subst. apply andp_right; try apply prop_right; auto.
+apply exp_right with 8.
 normalize.
-repeat apply andp_right; try apply prop_right.
-compute; congruence.
-compute; congruence.
 cancel.
 simpl_typed_mapsto.
 simpl.
@@ -131,12 +161,12 @@ name buf0 _buf.
 name x _x.
 name y _y.
 name len0 _length.
-change 8 with (sizeof t_struct_intpair).
+change (mf_size intpair_message) with (sizeof t_struct_intpair).
 rewrite memory_block_typed.
 do 2 simpl_typed_mapsto.
 destruct data as (x1,y1); simpl in *.
 apply semax_pre_PQR with
- (PROP  (isptr buf)
+ (PROP  (isptr buf; len=8)
    LOCAL  (`(eq p) (eval_id _p); `(eq buf) (eval_id _buf); `(eq (Vint (Int.repr len))) (eval_id _length))
    SEP 
    (`(field_mapsto_ sh t_struct_intpair _x) (eval_id _p);
@@ -147,7 +177,9 @@ apply semax_pre_PQR with
    `(mapsto sh' tint)
         (`(add_ptr_int tint) (`(eval_cast (tptr tuchar) (tptr tint)) (eval_id _buf)) `1)
         `(Vint y1))).
-go_lower; subst. rewrite field_mapsto_isptr. normalize.
+go_lower; subst.
+simpl_typed_mapsto. simpl.
+ rewrite field_mapsto_isptr. normalize.
  cancel.
 apply sepcon_derives; apply derives_refl'';
  eapply mapsto_field_mapsto; unfold field_offset; try (simpl; reflexivity);
@@ -168,7 +200,7 @@ cancel.
 rewrite sepcon_comm.
 apply sepcon_derives;
 apply derives_refl'; eapply mapsto_field_mapsto;  unfold field_offset; try (simpl; reflexivity);
- destruct buf0; inv H0; unfold eval_binop; simpl; reflexivity.
+ destruct buf0; inv H1; unfold eval_binop; simpl; reflexivity.
 Qed.
 
 Ltac simpl_stackframe_of := 
@@ -232,7 +264,7 @@ LOCAL ()
        (eval_var _intpair_deserialize
           (globtype (Global_func (deserialize_spec intpair_message)))) &&
      main_pre prog u) :: XX)) |-- PROP  ()  LOCAL ()  
-                                                   (SEPx (`(message intpair_message Ews)  (eval_var _intpair_message t_struct_message)
+                                                   (SEPx (`(message Ews intpair_message)  (eval_var _intpair_message t_struct_message)
                 :: XX)).
 Proof.
 intros.
@@ -352,7 +384,6 @@ match goal with |- semax _ (PROPx _ (LOCALx _ (SEPx (?R1::_)))) _ _ =>
  let H := fresh in assert (H: R1 = R); [ | rewrite H; clear H]
 end.
 
-
 Lemma call_serialize:
  forall (Delta: tycontext) P Q R (ser id x: ident)
            (sh_obj : share) (e_obj: expr) (d_obj: environ -> val)
@@ -366,15 +397,15 @@ Lemma call_serialize:
  writable_share sh_buf ->
  closed_wrt_vars (modified2 (modified1 ser) (modified1 x)) 
              (PROPx P (LOCALx Q
-     (SEPx (`(message msg sh_obj) d_obj :: 
-               `(typed_mapsto t sh_p) d_p `v::
-               `(typed_mapsto_ sh_buf (tarray tuchar (fst msg))) d_buf ::
+     (SEPx (`(message sh_obj msg) d_obj :: 
+               `(typed_mapsto sh_p t) d_p `v::
+               `(typed_mapsto_ sh_buf (tarray tuchar (mf_size msg))) d_buf ::
                 R)))) ->
  semax Delta
    (PROPx P (LOCALx Q
-     (SEPx (`(message msg sh_obj) d_obj :: 
-               `(typed_mapsto t sh_p) d_p `v::
-               `(typed_mapsto_ sh_buf (tarray tuchar (fst msg))) d_buf ::
+     (SEPx (`(message sh_obj msg) d_obj :: 
+               `(typed_mapsto sh_p t) d_p `v::
+               `(typed_mapsto_ sh_buf (tarray tuchar (mf_size msg))) d_buf ::
                 R))))
    (Ssequence 
     (Sset ser 
@@ -382,17 +413,74 @@ Lemma call_serialize:
         (tptr (Tfunction (Tcons (tptr tvoid) (Tcons (tptr tuchar) Tnil)) tint))))
       (Ssequence
            (Scall (Some x)
-              (Etempvar _ser (tptr (Tfunction (Tcons (tptr tvoid) (Tcons (tptr tuchar) Tnil)) tint)))
+              (Etempvar ser (tptr (Tfunction (Tcons (tptr tvoid) (Tcons (tptr tuchar) Tnil)) tint)))
               (e_p :: e_buf :: nil))
            (Sset id (Etempvar x tint))))
     (normal_ret_assert (PROPx P (LOCALx Q
-     (SEPx (`(message msg sh_obj) d_obj :: 
-               `(typed_mapsto t Share.top) d_p `v::
-               `(snd msg sh_buf) d_buf `v::
+     (SEPx (`(message sh_obj msg) d_obj :: 
+               `(typed_mapsto sh_p t) d_p `v::
+               `(mf_assert msg sh_buf) d_buf (`Int.signed (`force_int (eval_id id))) `v::
+               `(mf_restbuf msg sh_buf) d_buf (`Int.signed (`force_int (eval_id id))) ::
                 R))))).
 Admitted.
-(* need to add a proof to message_format, that the
-     representation of a  buf implies the typed_mapsto_ of the bufsize array *)
+
+Lemma call_deserialize:
+ forall (Delta: tycontext) P Q R (ser: ident)
+           (sh_obj : share) (e_obj: expr) (d_obj: environ -> val)
+           (sh_p: share) (e_p: expr) (d_p: environ -> val)
+           (sh_buf: share) (e_buf: expr) (d_buf: environ -> val)
+           (e_len: expr)  (d_len: environ -> Z) (t: type) (msg: message_format t)   (v: reptype t),
+ eval_lvalue e_obj = d_obj ->
+ eval_expr e_p = d_p ->
+ eval_expr e_buf = d_buf ->
+ writable_share sh_p ->
+  (PROPx P (LOCALx Q
+     (SEPx (`(message sh_obj msg) d_obj :: 
+               `(typed_mapsto_ sh_p t) d_p::
+               `(mf_assert msg sh_buf) d_buf d_len `v ::
+                R)))) |-- local (`(fun n => 0 <= n <= mf_size msg) d_len) &&
+                             local (`eq d_len (`Int.signed (`force_int (eval_expr e_len)))) ->
+ closed_wrt_vars (modified1 ser)
+             (PROPx P (LOCALx Q
+     (SEPx (`(message sh_obj msg) d_obj :: 
+               `(typed_mapsto_ sh_p t) d_p::
+               `(mf_assert msg sh_buf) d_buf d_len `v ::
+                R)))) ->
+ semax Delta
+   (PROPx P (LOCALx Q
+     (SEPx (`(message sh_obj msg) d_obj :: 
+               `(typed_mapsto_ sh_p t) d_p::
+               `(mf_assert msg sh_buf) d_buf d_len`v ::
+                R))))
+   (Ssequence 
+    (Sset ser 
+     (Efield e_obj _deserialize 
+        (tptr  (Tfunction (Tcons (tptr tvoid) (Tcons (tptr tuchar) (Tcons tint Tnil))) tvoid))))
+      (Scall None
+        (Etempvar ser (tptr  (Tfunction (Tcons (tptr tvoid) (Tcons (tptr tuchar) (Tcons tint Tnil))) tvoid)))
+          (e_p :: e_buf :: e_len :: nil)))
+    (normal_ret_assert (PROPx P (LOCALx Q
+     (SEPx (`(message sh_obj msg) d_obj :: 
+               `(typed_mapsto sh_p t) d_p `v::
+               `(mf_assert msg sh_buf) d_buf d_len`v::
+                R))))).
+Admitted.
+
+Lemma intpair_message_length:
+  forall sh p (len: environ -> Z) v P Q R,
+    (PROPx P (LOCALx Q (SEPx
+       (`(mf_assert intpair_message sh) p len v :: R)))) |--
+   (PROPx P 
+        (LOCALx (`(eq (mf_size intpair_message)) len :: Q)
+         (SEPx (`(mf_assert intpair_message sh) p len v :: R)))).
+Proof.
+intros.
+change SEPx with SEPx'; 
+unfold PROPx, LOCALx, SEPx', local; intro rho; simpl.
+apply andp_derives; auto.
+unfold_coerce.
+normalize.
+Qed.
 
 Lemma body_main:  semax_body Vprog Gtot f_main main_spec.
 Proof.
@@ -420,7 +508,7 @@ apply drop_local.  (* tempory, should fix store_field_tac *)
 simpl app.
 simpl update_tycon. (* should forward do this? *)
 gather_SEP 2%nat.
-replace_SEP  (`(typed_mapsto t_struct_intpair Share.top)
+replace_SEP  (`(typed_mapsto Share.top t_struct_intpair)
                       (eval_var _p t_struct_intpair) `((Int.repr 1, Int.repr 2)) : assert).
 simpl_typed_mapsto.
 extensionality rho; unfold_coerce; simpl; rewrite sepcon_comm; reflexivity.
@@ -430,16 +518,46 @@ eapply semax_seq'.
 focus_SEP 1%nat.
 apply call_serialize; auto 50 with closed.
 simpl update_tycon.
-forward. (* ser = intpair_message.serialize; *)
 redefine_Delta.
-simpl eval_lvalue.
-autorewrite with subst.
+focus_SEP 2%nat.
+eapply semax_pre0; [apply intpair_message_length | ].
+focus_SEP 4%nat.
+focus_SEP 2%nat.
+rewrite -> seq_assoc.
+eapply semax_seq'.
+apply call_deserialize; auto 50 with closed.
+go_lower. apply andp_right; apply prop_right.
+simpl in H. omega. simpl in *. rewrite <- H.  reflexivity. 
+focus_SEP 1%nat.
+replace_SEP 
+  ((`(field_mapsto Share.top t_struct_intpair _x) (eval_var _q t_struct_intpair) `(Vint (Int.repr 1)) *
+   `(field_mapsto Share.top t_struct_intpair _y) (eval_var _q t_struct_intpair) `(Vint (Int.repr 2)))
+    : assert).
+reflexivity.
+flatten_sepcon_in_SEP.
+forward. (* x = q.x; *)
+forward. (* y = q.y; *)
+forward. (* return x+y; *)
+go_lower. subst. simpl. normalize. unfold main_post.
+ simpl in H2. rewrite <- H2.
+ unfold mf_restbuf; simpl. rewrite memory_block_zero. rewrite sepcon_emp.
 
-
-
-
-
-
+repeat rewrite <- sepcon_assoc.
+apply derives_trans with
+( typed_mapsto_ Share.top t_struct_intpair
+      (eval_var _q t_struct_intpair rho) 
+ * TT 
+ * typed_mapsto_ Share.top (tarray tuchar 8)
+      (eval_var _buf (tarray tuchar 8) rho)
+ *  typed_mapsto_ Share.top t_struct_intpair
+      (eval_var _p t_struct_intpair rho)).
+repeat apply sepcon_derives; auto.
+simpl_typed_mapsto; simpl. rewrite sepcon_comm; apply sepcon_derives; auto.
+rewrite <- memory_block_typed.
+change (sizeof (tarray tuchar 8)) with (sizeof t_struct_intpair).
+rewrite memory_block_typed. auto.
+cancel.
+Qed.
 
 
 
